\documentclass[12pt]{article}

\usepackage{fancyhdr} 
\usepackage{amsfonts}
\usepackage{amsmath}
\usepackage{amsthm}
\usepackage{dsfont}

\pagestyle{fancy}
\fancyhf{}
\rhead{Shaw \space \thepage}

\setlength\parindent{0pt}

\begin{document}
\thispagestyle{empty}
	
\begin{flushright}
Sage Shaw \\
m565 - Fall 2017 \\
Sep. 9, 2017
\end{flushright}
	
{\large \textbf{HW 1:XXXXXXXX}}\bigbreak

%problem 1.d
\hspace{-4 ex}\textbf{1 (d) } Show that for any $a_{0} > b_{0} > 0$ that $\{a_{n}\}$ and $\{b_{n}\}$ converge quadratically to
	some number which we will call $M(a_{0}, b_{0})$. \\
	
	\begin{proof}
		Since $a_{0} > b_{0}$, $a_{1} = \frac{1}{2} (a_{0}+b_{0}) < \frac{1}{2} (a_{0}+a_{0}) = a_{0}$. \\
		Thus $a_{1} < a_{0}$. \\
		Also note $b_{1}^{2} = a_{0}b_{0} > b_{0}^{2}$. Since both sides are positive, $b_{1} > b_{0}$. \\
		Now we show that $b_1<a_1$ as follows:\\
		\begin{align*}
			2a_1 & = a_0 + b_0 \\
			4a_1^2 & = a_0^2 + 2a_0b_0 + b_0^2 \\
			4a_1^2 - 4a_0b_0 & = a_0^2 - 2a_0b_0 + b_0^2 \\
			4(a_1^2 - a_0b_0) & = (a_0 - b_0)^2 > 0\\
			a_1^2 - a_0b_0 & > 0 \\
			a_1^2 - b_1^2 & > 0\\
			a_1 & > b_1\\
		\end{align*}
				
		We now have $0 < b_{0}< b_1 <a_{1} < a_{0}$ which will be our base case. \bigbreak
		
		Now we assume that $0< b_n <a_{n}$ for some $n \in \mathbb{N}$.\\
		Since $b_n < a_n$, $a_{n+1} = \frac{1}{2} (a_{n}+b_{n}) < \frac{1}{2} (a_{n}+a_{n}) = a_{n}$. \\
		Thus $a_{n+1} < a_{n}$. \\
		Also note $b_{n+1}^{2} = a_{n}b_{n} > b_{n}^{2}$. Since both sides are positive, $b_{n+1} > b_{n}$. \\
		Now we show that $b_{n+1}<a_{n+1}$ as follows:\\
		\begin{align*}
		2a_{n+1} & = a_n + b_n \\
		4a_{n+1}^2 & = a_n^2 + 2a_nb_n + b_n^2 \\
		4a_{n+1}^2 - 4a_nb_n & = a_n^2 - 2a_nb_n + b_n^2 \\
		4(a_{n+1}^2 - a_nb_n) & = (a_n - b_n)^2 > 0\\
		a_{n+1}^2 - a_nb_n & > 0 \\
		a_{n+1}^2 - b_{n+1}^2 & > 0\\
		a_{n+1} & > b_{n+1}\\
		\end{align*}
		
		\bigbreak
		
		By induction we have that $b_{n}<b_{n+1}<a_{n+1} < a_{n}$ for all $n \in \mathbb{N}$. \bigbreak
		
		Thus ${a_n}$ is monotonically decreasing and bounded below by $b_0$ and is thus convergent. \\
		Similarly ${b_n}$ is monotonically increasing and bounded above by $a_0$ and is thus convergent. \bigbreak
		
		We now show that $\lim\limits_{n \to \infty}a_n = \lim\limits_{n \to \infty}b_n$. \\
		Note that since $\{a_n\}$ is convergent, it is Cauchy: $\lim\limits_{n \to \infty}\vert a_n - a_{n+1} \vert = 0$. \\
		Also note that $a_{n+1} = \frac{1}{2}(a_n + b_n)$ can be rewritten as $b_n = 2a_{n+1} - a_{n}$. \\
		Then \\
		\begin{align*}
			\lim\limits_{n \to \infty} a_n - \lim\limits_{n \to \infty} b_n  &= \lim\limits_{n \to \infty}\vert a_n - b_n \vert  \\
			& = \lim\limits_{n \to \infty} \vert a_n - 2a_{n+1} + a_{n} \vert  \\
			& = 2\lim\limits_{n \to \infty} \vert a_n - a_{n+1} \vert \\
			& = 0 \\
			\lim\limits_{n \to \infty} a_n & = \lim\limits_{n \to \infty} b_n
		\end{align*}
		
		Define $M(a_{0}, b_{0}) = \lim\limits_{n \to \infty} a_n = \lim\limits_{n \to \infty} b_n$. \bigbreak
		
		We now show that the sequences converge quadratically. by considering the sequence $\{a_n-b_n\} \to 0$. \bigbreak
		
		Let $M = M(a_{0}, b_{0})$. Then \\
		\begin{align*}
			\lim\limits_{n \to \infty} \frac{\vert a_{n+1} - b_{n+1} - 0\vert}{ \vert a_n - b_n - 0 \vert ^ 2} & = \lim\limits_{n \to \infty} \frac{a_{n+1}-b_{n+1}}{(a_n -b_n) ^ 2} \\
			& = \lim\limits_{n \to \infty} \frac{ \frac{1}{2}(a_n+b_n) - \sqrt{a_nb_n}}{(a_n -b_n) ^ 2} \\
			& = \frac{1}{2} \lim\limits_{n \to \infty} \frac{a_n + b_n - 2\sqrt{a_nb_n}}{(a_n -b_n) ^ 2} \\
			& = \frac{1}{2} \lim\limits_{n \to \infty} \frac{(a_n + b_n) - 2\sqrt{a_nb_n}}{(a_n -b_n) ^ 2} * \frac{(a_n + b_n) + 2\sqrt{a_nb_n}}{(a_n + b_n) + 2\sqrt{a_nb_n}}\\
			& = \frac{1}{2} \lim\limits_{n \to \infty} \frac{(a_n + b_n)^2 - 4a_nb_n}{(a_n -b_n) ^ 2 \big( (a_n + b_n) + 2\sqrt{a_nb_n} \big) } \\
			& = \frac{1}{2} \lim\limits_{n \to \infty} \frac{a_n^2 + 2a_nb_n + b_n^2 - 4a_nb_n}{(a_n -b_n) ^ 2 \big( (a_n + b_n) + 2\sqrt{a_nb_n} \big) } \\
			& = \frac{1}{2} \lim\limits_{n \to \infty} \frac{a_n^2 - 2a_nb_n + b_n^2}{(a_n -b_n) ^ 2 \big( (a_n + b_n) + 2\sqrt{a_nb_n} \big) } \\
			& = \frac{1}{2} \lim\limits_{n \to \infty} \frac{(a_n -b_n) ^ 2}{(a_n -b_n) ^ 2 \big( (a_n + b_n) + 2\sqrt{a_nb_n} \big) } \\
			& = \frac{1}{2} \lim\limits_{n \to \infty} \frac{1}{ a_n + b_n + 2\sqrt{a_nb_n} } \\
			& = \frac{1}{2} \frac{1}{ M + M + 2\sqrt{MM} } \\
			& = \frac{1}{8M}
		\end{align*}
		
		Since $ a_n - M < a_n - b_n$ we can say that $\{a_n\}$ converges quadratically, and since $b_n - M < b_n - a_n$, we can say that $\{b_n\}$ converges quadratically as well, both with convergence constant $\lambda = \frac{1}{8M}$. \\
		
		
		
		
		 
	\end{proof}

\end{document}
